[Bulgaria1998P1] clean up problem statement

Compfiles/Bulgaria1998P1.lean
@@ -15,25 +15,50 @@ problem_file
 /-!
 Bulgarian Mathematical Olympiad 1998, Problem 1
 
-Find the least natural number n (n ≥ 3) with the following property:
-for any coloring in 2 colors of n distinct collinear points A₁, A₂, ..., Aₙ,
-there exist three points Aᵢ, Aⱼ, A₂ⱼ₋ᵢ, 1 ≤ i < 2j - i ≤ n, which are colored
-the same color.
+We will be considering colorings in 2 colors of n (distinct) points
+A₁, A₂, ..., Aₙ. Call such a coloring "good" if there exist three points
+Aᵢ, Aⱼ, A₂ⱼ₋ᵢ, 1 ≤ i < 2j - i ≤ n, which are colored the same color.
+
+Find the least natural number n (n ≥ 3) such that all colorings
+of n points are good.
 -/
 
 namespace Bulgaria1998P1
 
-def coloring_has_desired_points (m : ℕ) (color : Set.Icc 1 m → Fin 2) : Prop :=
+abbrev coloring_is_good {m : ℕ} (color : Set.Icc 1 m → Fin 2) : Prop :=
   ∃ i j : Set.Icc 1 m,
     i < j ∧
     ∃ h3 : 2 * j.val - i ∈ Set.Icc 1 m,
     color i = color j ∧ color i = color ⟨2 * j - i, h3⟩
 
-determine n : ℕ := 9
+abbrev all_colorings_are_good (m : ℕ) : Prop :=
+  3 ≤ m ∧ ∀ color : Set.Icc 1 m → Fin 2, coloring_is_good color
 
 snip begin
 
-def coloring_of_eight : Set.Icc 1 8 → Fin 2
+lemma lemma1 {m n : ℕ} (hmn : m ≤ n) (hm : all_colorings_are_good m) :
+    all_colorings_are_good n := by
+  constructor
+  · exact hm.1.trans hmn
+  · intro c
+    let c' : Set.Icc 1 m → Fin 2 :=
+      fun x ↦ c ⟨x.val, by rw [Set.mem_Icc]; exact ⟨x.prop.1, x.prop.2.trans hmn⟩⟩
+    obtain ⟨⟨i, hi1, hi2⟩, ⟨j, hj1, hj2⟩, hij1, hij2, hc1, hc2⟩ := hm.2 c'
+    use ⟨i, hi1, hi2.trans hmn⟩
+    use ⟨j, hj1, hj2.trans hmn⟩
+    simp only [Subtype.mk_lt_mk, Nat.lt_one_iff, Set.mem_Icc,
+               tsub_le_iff_right, exists_and_left]
+    simp only [Subtype.mk_lt_mk] at hij1
+    refine' ⟨hij1, _⟩
+    simp only [Nat.lt_one_iff, Set.mem_Icc, tsub_le_iff_right] at hij2
+    unfold_let c' at hc1
+    simp only at hc1
+    refine' ⟨hc1, _⟩
+    have hij2' : 1 ≤ 2 * j - i ∧ 2 * j ≤ n + i :=
+       ⟨hij2.1, le_add_of_le_add_right hij2.2 hmn⟩
+    use hij2'
+
+def coloring_of_eight {n : ℕ} : Set.Icc 1 n → Fin 2
 | ⟨1, _⟩ => 0
 | ⟨2, _⟩ => 1
 | ⟨3, _⟩ => 0
@@ -44,17 +69,29 @@ def coloring_of_eight : Set.Icc 1 8 → Fin 2
 | ⟨8, _⟩ => 0
 | _ => 0 -- unreachable
 
-snip end
-
-problem bulgaria1998_p1a :
-    ∃ f: Set.Icc 1 (n - 1) → Fin 2, ¬coloring_has_desired_points (n - 1) f := by
+lemma lemma2 :
+    ∃ f : Set.Icc 1 8 → Fin 2, ¬coloring_is_good f := by
   use coloring_of_eight
   intro h
   obtain ⟨⟨i, hi1, hi2⟩, ⟨j, hj1, hj2⟩, hij1, hij2, hc1, hc2⟩ := h
-  have hn1 : n - 1 = 8 := by simp[n]
-  rw [hn1] at hi2 hj2
   dsimp [coloring_of_eight] at *
   interval_cases i <;> interval_cases j <;> aesop
 
-problem bulgaria1998_p1b (color : Set.Icc 1 n → Fin 2) : coloring_has_desired_points n f := by
-  sorry
+snip end
+
+determine solution_data : ℕ := 9
+
+problem bulgaria1998_p1 : IsLeast { m | all_colorings_are_good m } solution_data := by
+  constructor
+  · rw [Set.mem_setOf_eq]
+    refine' ⟨by norm_num, _⟩
+    intro color
+    sorry
+  · rw [mem_lowerBounds]
+    intro n hn
+    rw [Set.mem_setOf_eq] at hn
+    by_contra' H
+    have h1 : n ≤ solution_data - 1 := Nat.le_pred_of_lt H
+    have ⟨h2, h3⟩ := lemma1 h1 hn
+    obtain ⟨f, hf⟩ := lemma2
+    exact (hf (h3 f)).elim
